EFComp1 checkpoint

src/ElimFuncComp1.v
@@ -1,96 +1,1159 @@
 Require Import Common Monads.
 Require Import Metadata.
 Require String.
-Require TaggedNumbered ElimFunc.
+Require Tagged.
 Require Import ListLemmas.
 Require Import StepLib.
 Require Import HigherValue.
 
 Require Import Psatz.
 
-Module A := TaggedNumbered.
-Module B := TaggedNumbered.
+Module A := Tagged.
+Module B := Tagged.
+
+Set Default Timeout 15.
 
 
-Definition compile base :=
+
+Definition nth_local n :=
+    match n with
+    | 0 => B.Arg
+    | S n => B.UpVar n
+    end.
+
+Fixpoint locals_list' n acc :=
+    match n with
+    | 0 => acc
+    | S n => locals_list' n (nth_local n :: acc)
+    end.
+
+Definition locals_list n := locals_list' n [].
+
+
+(* Increment all variable references by `n`. *)
+
+Definition shift n :=
     let fix go e :=
         let fix go_list es :=
             match es with
             | [] => []
             | e :: es => go e :: go_list es
             end in
-        match e with
-        | A.Value v => B.Value v
-        | A.Arg => B.Arg
-        | A.UpVar n => B.UpVar n
-        | A.Call f a => B.Call (go f) (go a)
-        | A.MkConstr tag args => B.MkConstr tag (go_list args)
-        | A.ElimN n cases target =>
-                let expect := A.num_locals_list_pair cases in
-                let func := B.MkCloseDyn (base + n) 0 expect in
-                B.Call func (go target)
-        | A.MkClose fname free => B.MkClose fname (go_list free)
-        end in go.
+        let go_pair p :=
+            let '(e, r) := p in
+            (go e, r) in
+        let fix go_list_pair ps :=
+            match ps with
+            | [] => []
+            | p :: ps => go_pair p :: go_list_pair ps
+            end in
 
-Definition compile_list base :=
-    let go := compile base in
+        match e with
+        | A.Value v => A.Value v
+        | A.Arg => A.UpVar n
+        | A.UpVar n' => A.UpVar (n + n')
+        | A.Call f a => A.Call (go f) (go a)
+        | A.MkConstr tag args => A.MkConstr tag (go_list args)
+        | A.Elim cases target => A.Elim (go_list_pair cases) (go target)
+        | A.MkClose fname free => A.MkClose fname (go_list free)
+        end
+    in go.
+
+Definition shift_list n :=
+    let go := shift n in
     let fix go_list es :=
         match es with
         | [] => []
         | e :: es => go e :: go_list es
         end in go_list.
 
-Ltac refold_compile base :=
-    fold (compile_list base) in *.
-
-Definition compile_pair base :=
-    let go := compile base in
+Definition shift_pair n :=
+    let go := shift n in
     let fix go_pair (p : A.expr * A.rec_info) :=
         let '(e, r) := p in
         (go e, r) in go_pair.
 
-Definition compile_list_pair base :=
-    let go_pair := compile_pair base in
+Definition shift_list_pair n :=
+    let go_pair := shift_pair n in
     let fix go_list_pair es :=
         match es with
         | [] => []
         | e :: es => go_pair e :: go_list_pair es
         end in go_list_pair.
 
+Ltac refold_shift n :=
+    fold (shift_list n) in *;
+    fold (shift_pair n) in *;
+    fold (shift_list_pair n) in *.
 
-Definition compile_eliminator base n cases :=
-    let expect := A.num_locals_list_pair cases in
-    let cases' := compile_list_pair base cases in
-    let rec := B.MkCloseDyn (base + n) 1 expect in
-    B.ElimBody rec cases'.
 
-Fixpoint compile_eliminator_list' base n elims :=
-    match elims with
-    | [] => []
-    | elim :: elims =>
-            compile_eliminator base n elim ::
-            compile_eliminator_list' base (S n) elims
+
+Section compile.
+
+Open Scope state_monad.
+
+Definition record (e : B.expr) (nfree : nat) : state (list (B.expr * nat)) nat :=
+    fun s => (length s, s ++ [(e, nfree)]).
+
+Notation pure := ret_state.
+
+(* `nfree` is the number of free variables in the original function.
+   `depth` is the number of `A.Elim`s we're currently under.  Each Elim is
+   lifted to a function, which binds an additional variable.
+ *)
+Definition compile base nfree : nat -> A.expr -> state _ B.expr :=
+    let fix go depth e {struct e} :=
+        let fix go_list depth es :=
+            match es with
+            | [] => pure []
+            | e :: es => @cons _ <$> go depth e <*> go_list depth es
+            end in
+        let go_pair depth p :=
+            let '(e, r) := p in
+            go depth e >>= fun e' => pure (e', r) in
+        let fix go_list_pair depth ps :=
+            match ps with
+            | [] => pure []
+            | p :: ps => @cons _ <$> go_pair depth p <*> go_list_pair depth ps
+            end in
+
+        match e with
+        | A.Value v => pure (B.Value v)
+        | A.Arg =>
+                match depth with
+                | 0 => pure (B.Arg)
+                | S n => pure (B.UpVar n)
+                end
+        | A.UpVar n => pure (B.UpVar (depth + n))
+        | A.Call f a => B.Call <$> go depth f <*> go depth a
+        | A.MkConstr tag args => B.MkConstr tag <$> go_list depth args
+        | A.Elim cases target =>
+                go_list_pair (S depth) cases >>= fun cases' =>
+                record (B.Elim cases' B.Arg) (S depth + nfree) >>= fun n =>
+                go depth target >>= fun target' =>
+                let func := B.MkClose (base + n) (locals_list (depth + nfree)) in
+                pure (B.Call func target')
+        | A.MkClose fname free => B.MkClose fname <$> go_list depth free
+        end in go.
+
+Definition compile_list base nfree : nat -> list A.expr -> state _ (list B.expr) :=
+    let go := compile base nfree in
+    let fix go_list depth es :=
+        match es with
+        | [] => pure []
+        | e :: es => @cons _ <$> go depth e <*> go_list depth es
+        end in go_list.
+
+Definition compile_pair base nfree : nat -> (A.expr * A.rec_info) -> state _ (B.expr * B.rec_info) :=
+    let go := compile base nfree in
+    let go_pair depth (p : A.expr * A.rec_info) :=
+        let '(e, r) := p in
+        go depth e >>= fun e' => pure (e', r)
+    in go_pair.
+
+Definition compile_list_pair base nfree :
+        nat -> list (A.expr * A.rec_info) -> state _ (list (B.expr * B.rec_info)) :=
+    let go_pair := compile_pair base nfree in
+    let fix go_list_pair depth ps :=
+        match ps with
+        | [] => pure []
+        | p :: ps => @cons _ <$> go_pair depth p <*> go_list_pair depth ps
+        end in go_list_pair.
+
+Lemma unfold_compile base nfree depth e :
+    compile base nfree depth e =
+    match e with
+    | A.Value v => pure (B.Value v)
+    | A.Arg =>
+            match depth with
+            | 0 => pure (B.Arg)
+            | S n => pure (B.UpVar n)
+            end
+    | A.UpVar n => pure (B.UpVar (depth + n))
+    | A.Call f a => B.Call <$> compile base nfree depth f <*> compile base nfree depth a
+    | A.MkConstr tag args => B.MkConstr tag <$> compile_list base nfree depth args
+    | A.Elim cases target =>
+            compile_list_pair base nfree (S depth) cases >>= fun cases' =>
+            record (B.Elim cases' B.Arg) (S depth + nfree) >>= fun n =>
+            compile base nfree depth target >>= fun target' =>
+            let func := B.MkClose (base + n) (locals_list (depth + nfree)) in
+            pure (B.Call func target')
+    | A.MkClose fname free => B.MkClose fname <$> compile_list base nfree depth free
+    end.
+revert e depth.
+mut_induction e using A.expr_rect_mut' with
+    (Pl := fun es => forall depth,
+        compile_list base nfree depth es =
+        match es with
+        | [] => pure []
+        | e :: es => @cons _ <$> compile base nfree depth e <*> compile_list base nfree depth es
+        end)
+    (Pp := fun p => forall depth,
+        compile_pair base nfree depth p =
+        let '(e, r) := p in
+        compile base nfree depth e >>= fun e' => pure (e', r))
+    (Plp := fun ps => forall depth,
+        compile_list_pair base nfree depth ps =
+        match ps with
+        | [] => pure []
+        | p :: ps => @cons _
+                <$> compile_pair base nfree depth p
+                <*> compile_list_pair base nfree depth ps
+        end);
+try solve [reflexivity].
+
+finish_mut_induction unfold_compile using list pair list_pair.
+Qed exporting.
+
+Fixpoint compile_cu' base exprs metas :=
+    match exprs, metas with
+    | [], [] => pure []
+    | e :: exprs, m :: metas =>
+            compile base (m_nfree m) 0 e >>= fun e' =>
+            compile_cu' base exprs metas >>= fun es' =>
+            pure (e' :: es')
+    | _, _ => pure []
     end.
 
-Definition compile_eliminator_list base elims :=
-    compile_eliminator_list' base 0 elims.
+End compile.
 
-Definition compile_env elims exprs :=
-    compile_list (length exprs) exprs ++
-    compile_eliminator_list (length exprs) elims.
+Opaque compile compile_list compile_pair compile_list_pair.
+Ltac unfold_compile_in H :=
+    first
+        [ rewrite 1!unfold_compile in H
+        | rewrite 1!unfold_compile_list in H
+        | rewrite 1!unfold_compile_pair in H
+        | rewrite 1!unfold_compile_list_pair in H
+        ].
 
-Definition compile_cu (cu :
-            list A.expr * list metadata *
-            list (list (A.expr * A.rec_info)) * list String.string) :
+Ltac refold_compile base nfree :=
+    fold (compile_list base nfree) in *;
+    fold (compile_pair base nfree) in *;
+    fold (compile_list_pair base nfree) in *.
+
+Fixpoint process_elims elims n : list B.expr * list metadata :=
+    match elims with
+    | [] => ([], [])
+    | (e, nfree) :: elims =>
+            let '(exprs, metas) := process_elims elims (S n) in
+            let name := String.append "__oeuf_elim" (nat_to_string n) in
+            (e :: exprs, Metadata name Private nfree :: metas)
+    end.
+
+Definition compile_cu (cu : list A.expr * list metadata) :
         option (list B.expr * list metadata) :=
-    let '(exprs, metas, elims, elim_names) := cu in
-    if eq_nat_dec (length exprs) (length metas) then
-        let exprs' := compile_list (length exprs) exprs in
-        let elims' := compile_eliminator_list (length exprs) elims in
-        let elim_metas := map (fun name => Metadata name Private) elim_names in
-        Some (exprs' ++ elims', metas ++ elim_metas)
-    else
-        NonB.
+    let '(exprs, metas) := cu in
+    let nfrees := map m_nfree metas in
+    let '(exprs'_base, elims) := compile_cu' (length exprs) exprs metas [] in
+    let (exprs'_elims, metas_elims) := process_elims elims 0 in
+    Some (exprs'_base ++ exprs'_elims, metas ++ metas_elims).
+
+
+Inductive I_expr (BE : B.env) nfree : nat -> A.expr -> B.expr -> Prop :=
+| IValue : forall depth v, I_expr BE nfree depth (A.Value v) (B.Value v)
+| IArg0 : I_expr BE nfree 0 A.Arg B.Arg
+| IArgS : forall depth, I_expr BE nfree (S depth) A.Arg (B.UpVar depth)
+| IUpVar : forall depth n, I_expr BE nfree depth (A.UpVar n) (B.UpVar (depth + n))
+| ICall : forall depth af aa bf ba,
+        I_expr BE nfree depth af bf ->
+        I_expr BE nfree depth aa ba ->
+        I_expr BE nfree depth (A.Call af aa) (B.Call bf ba)
+| IMkConstr : forall depth tag aargs bargs,
+        Forall2 (I_expr BE nfree depth) aargs bargs ->
+        I_expr BE nfree depth (A.MkConstr tag aargs) (B.MkConstr tag bargs)
+| IElim : forall depth acases atarget bcases btarget,
+        Forall2 (fun ap bp => I_expr BE nfree depth (fst ap) (fst bp) /\
+                snd ap = snd bp) acases bcases ->
+        I_expr BE nfree depth atarget btarget ->
+        I_expr BE nfree depth (A.Elim acases atarget) (B.Elim bcases btarget)
+| IMkClose : forall depth fname aargs bargs,
+        Forall2 (I_expr BE nfree depth) aargs bargs ->
+        I_expr BE nfree depth (A.MkClose fname aargs) (B.MkClose fname bargs)
+| IElimCall : forall depth acases atarget bcases btarget bfname,
+        Forall2 (fun ap bp => I_expr BE nfree (S depth) (fst ap) (fst bp) /\
+                snd ap = snd bp) acases bcases ->
+        I_expr BE nfree depth atarget btarget ->
+        nth_error BE bfname = Some (B.Elim bcases B.Arg) ->
+        I_expr BE nfree depth
+                (A.Elim acases atarget)
+                (B.Call (B.MkClose bfname (locals_list (depth + nfree))) btarget)
+.
+
+Inductive I (AE : A.env) (BE : B.env) : A.state -> B.state -> Prop :=
+| IRun : forall ae al ak be bextra bl bk nfree,
+        I_expr BE nfree (length bextra) ae be ->
+        (forall v,
+            I AE BE (ak v) (bk v)) ->
+        length al = nfree ->
+        bextra ++ al = bl ->
+        I AE BE (A.Run ae al ak) (B.Run be bl bk)
+
+| IMidElim : forall acases al ak bfname bcases bextra bl bk target nfree,
+        (* This is the state where we've finished evaluating the elim target on
+           both sides, but haven't entered a case yet. *)
+        Forall2 (fun ap bp => I_expr BE nfree (S (length bextra)) (fst ap) (fst bp) /\
+                snd ap = snd bp) acases bcases ->
+        nth_error BE bfname = Some (B.Elim bcases B.Arg) ->
+
+        length al = nfree ->
+        bextra ++ al = bl ->
+        (forall v,
+            I AE BE (ak v) (bk v)) ->
+
+        I AE BE
+            (A.Run (A.Elim acases (A.Value target)) al ak)
+            (B.Run (B.Call (B.Value (Close bfname bl)) (B.Value target)) bl bk)
+
+| IStop : forall v,
+        I AE BE (A.Stop v) (B.Stop v).
+
+
+
+
+
+Ltac spec_assert H :=
+    match type of H with
+    | forall x : ?T, _ =>
+            assert (HH : T); [ | specialize (H HH); try clear HH ]
+    end.
+
+Lemma Forall2_imp : forall {A B} (P Q : A -> B -> Prop) xs ys,
+    Forall2 P xs ys ->
+    (forall x y, P x y -> Q x y) ->
+    Forall2 Q xs ys.
+induction xs; destruct ys; intros0 Hfa Himp; invc Hfa; econstructor; eauto.
+Qed.
+
+Lemma Forall2_conj : forall {A B} (P Q : A -> B -> Prop) xs ys,
+    Forall2 P xs ys ->
+    Forall2 Q xs ys ->
+    Forall2 (fun x y => P x y /\ Q x y) xs ys.
+induction xs; destruct ys; intros0 Hfa1 Hfa2; invc Hfa1; invc Hfa2; econstructor; eauto.
+Qed.
+
+Lemma Forall2_conj_inv : forall A B (P Q : A -> B -> Prop) xs ys (M : Prop),
+    (Forall2 P xs ys ->
+        Forall2 Q xs ys ->
+        M) ->
+    Forall2 (fun x y => P x y /\ Q x y) xs ys -> M.
+intros0 HM Hfa.
+eapply HM; eapply Forall2_imp with (1 := Hfa); intros; firstorder.
+Qed.
+
+
+
+Lemma nth_error_app_Some : forall A (xs ys : list A) n x,
+    nth_error xs n = Some x ->
+    nth_error (xs ++ ys) n = Some x.
+intros. rewrite nth_error_app1; eauto.
+eapply nth_error_Some. congruence.
+Qed.
+
+
+Lemma I_expr_weaken : forall BE BE' nfree depth ae be,
+    I_expr BE nfree depth ae be ->
+    I_expr (BE ++ BE') nfree depth ae be.
+intros ? ? ? ?.
+intro ae. revert ae depth.
+mut_induction ae using A.expr_rect_mut' with
+    (Pl := fun aes => forall depth bes,
+        Forall2 (I_expr BE nfree depth) aes bes ->
+        Forall2 (I_expr (BE ++ BE') nfree depth) aes bes)
+    (Pp := fun (ap : A.expr * A.rec_info) => forall (bp : B.expr * B.rec_info) depth,
+        I_expr BE nfree depth (fst ap) (fst bp) ->
+        I_expr (BE ++ BE') nfree depth (fst ap) (fst bp))
+    (Plp := fun (aps : list (A.expr * A.rec_info)) =>
+        forall (bps : list (B.expr * B.rec_info)) depth,
+        Forall2 (fun ap bp => I_expr BE nfree depth (fst ap) (fst bp)) aps bps ->
+        Forall2 (fun ap bp => I_expr (BE ++ BE') nfree depth (fst ap) (fst bp)) aps bps);
+intros0 II.
+
+- invc II. econstructor.
+- invc II; econstructor.
+- invc II. econstructor.
+- invc II. econstructor; eauto.
+- invc II. econstructor; eauto.
+- invc II.
+  + econstructor; eauto.
+    on (Forall2 _ _ _), invc_using Forall2_conj_inv.
+    eapply Forall2_conj; eauto.
+  + econstructor; eauto; cycle 1.
+      { eapply nth_error_app_Some. eassumption. }
+    on (Forall2 _ _ _), invc_using Forall2_conj_inv.
+    eapply Forall2_conj; eauto.
+- invc II. econstructor; eauto.
+
+- invc II. econstructor.
+- invc II. econstructor; eauto.
+
+- destruct bp. simpl in *. eauto.
+
+- invc II. econstructor.
+- invc II. econstructor; eauto.
+
+- finish_mut_induction I_expr_weaken using list pair list_pair.
+Qed exporting.
+
+Lemma record_state_monotonic : forall e nfree s n s',
+    record e nfree s = (n, s') ->
+    exists s1, s' = s ++ s1.
+intros0 Hrec. unfold record in *. invc Hrec. eauto.
+Qed.
+
+Lemma record_nth_error : forall e nfree s n s',
+    record e nfree s = (n, s') ->
+    nth_error s' n = Some (e, nfree).
+intros0 Hrec. unfold record in *. invc Hrec.
+rewrite nth_error_app2; eauto.
+replace (_ - _) with 0 by omega. reflexivity.
+Qed.
+
+
+Lemma compile_state_monotonic : forall base nfree depth e s e' s',
+    compile base nfree depth e s = (e', s') ->
+    exists s1, s' = s ++ s1.
+intros0 HH. revert e depth e' s s' HH.
+mut_induction e using A.expr_rect_mut' with
+    (Pl := fun es => forall depth es' s s',
+        compile_list base nfree depth es s = (es', s') ->
+        exists s1, s' = s ++ s1)
+    (Pp := fun (p : A.expr * A.rec_info) => forall depth (p' : B.expr * B.rec_info) s s',
+        compile_pair base nfree depth p s = (p', s') ->
+        exists s1, s' = s ++ s1)
+    (Plp := fun (ps : list (A.expr * A.rec_info)) =>
+        forall depth (ps' : list (B.expr * B.rec_info)) s s',
+        compile_list_pair base nfree depth ps s = (ps', s') ->
+        exists s1, s' = s ++ s1);
+[ intros0 Hcomp; unfold_compile_in Hcomp.. | ].
+
+- break_bind_state. exists []. eauto using app_nil_r.
+- break_match; break_bind_state.
+  all: exists []; eauto using app_nil_r.
+- break_bind_state. exists []. eauto using app_nil_r.
+
+- (* Call *) break_bind_state.
+  specialize (IHe1 ?? ?? ?? ?? ** ).
+  specialize (IHe2 ?? ?? ?? ?? ** ).
+  do 2 break_exists. eexists.
+  do 2 on _, fun H => rewrite H.
+  rewrite <- app_assoc. reflexivity.
+
+- break_bind_state. eauto.
+
+- (* Elim *) break_bind_state.
+  specialize (IHe ?? ?? ?? ?? ** ).
+  specialize (IHe0 ?? ?? ?? ?? ** ).
+  pose proof (record_state_monotonic ?? ?? ?? ?? ?? ** ).
+  do 3 break_exists. eexists.
+  rewrite H0, H, H1. do 2 rewrite <- app_assoc. reflexivity.
+
+- break_bind_state. eauto.
+
+(* list *)
+- break_bind_state. exists []. eauto using app_nil_r.
+- break_bind_state.
+  specialize (IHe ?? ?? ?? ?? ** ).
+  specialize (IHe0 ?? ?? ?? ?? ** ).
+  do 2 break_exists. eexists.
+  do 2 on _, fun H => rewrite H.
+  rewrite <- app_assoc. reflexivity.
+
+(* pair *)
+- break_bind_state. eauto.
+
+(* list_pair *)
+- break_bind_state. exists []. eauto using app_nil_r.
+- break_bind_state.
+  specialize (IHe ?? ?? ?? ?? ** ).
+  specialize (IHe0 ?? ?? ?? ?? ** ).
+  do 2 break_exists. eexists.
+  do 2 on _, fun H => rewrite H.
+  rewrite <- app_assoc. reflexivity.
+
+- finish_mut_induction compile_state_monotonic using list pair list_pair.
+Qed exporting.
+
+Theorem compile_I_expr : forall BE0 nfree depth e s e' s',
+    compile (length BE0) nfree depth e s = (e', s') ->
+    I_expr (BE0 ++ map fst s') nfree depth e e'.
+intros BE0 nfree depth e. revert e depth.
+induction e using A.expr_rect_mut with
+    (Pl := fun es => forall depth s es' s',
+        compile_list (length BE0) nfree depth es s = (es', s') ->
+        Forall2 (I_expr (BE0 ++ map fst s') nfree depth) es es')
+    (Pp := fun p => forall depth s p' s',
+        compile_pair (length BE0) nfree depth p s = (p', s') ->
+        I_expr (BE0 ++ map fst s') nfree depth (fst p) (fst p') /\ snd p = snd p')
+    (Plp := fun ps => forall depth s ps' s',
+        compile_list_pair (length BE0) nfree depth ps s = (ps', s') ->
+        Forall2 (fun p p' => I_expr (BE0 ++ map fst s') nfree depth (fst p) (fst p') /\
+            snd p = snd p') ps ps');
+intros0 Hcomp; try (unfold_compile_in Hcomp; invc Hcomp).
+
+- (* Value *) econstructor.
+- (* Arg *)
+  destruct depth.
+  + on (ret_state _ _ = _), invc. econstructor.
+  + on (ret_state _ _ = _), invc. econstructor.
+- (* UpVar *) econstructor.
+
+- (* Call *)
+  break_bind_state.
+
+  rename s0 into s1, s into s0, s' into s2.
+  assert (HH : exists s01, s1 = s0 ++ s01) by (eapply compile_state_monotonic; eauto).
+    destruct HH as [s01 Hs01].
+  assert (HH : exists s12, s2 = s1 ++ s12) by (eapply compile_state_monotonic; eauto).
+    destruct HH as [s12 Hs12].
+  subst.
+
+  econstructor.
+  + rewrite map_app. rewrite app_assoc. eapply I_expr_weaken. eapply IHe1. eauto.
+  + eapply IHe2. eauto.
+
+- (* MkConstr *) break_bind_state.  econstructor. eapply IHe. eauto.
+
+- (* Elim *) break_bind_state.
+
+  rename s' into s3, s1 into s2, s0 into s1, s into s0.
+  assert (HH : exists s01, s1 = s0 ++ s01) by (eapply compile_state_monotonic_list_pair; eauto).
+    destruct HH as [s01 Hs01].
+  assert (HH : exists s12, s2 = s1 ++ s12) by (eapply record_state_monotonic; eauto).
+    destruct HH as [s12 Hs12].
+  assert (HH : exists s23, s3 = s2 ++ s23) by (eapply compile_state_monotonic; eauto).
+    destruct HH as [s23 Hs23].
+  subst.
+
+  econstructor.
+  + specialize (IHe ?? ?? ?? ?? ** ). invc_using Forall2_conj_inv IHe.
+    eapply Forall2_conj; eauto.
+    rewrite ?map_app, ?app_assoc. do 2 eapply I_expr_weaken_list_pair.
+    rewrite <- app_assoc, <- map_app. eauto.
+  + eapply IHe0. eassumption.
+  + rewrite ?map_app, app_assoc. eapply nth_error_app_Some.
+    rewrite nth_error_app2 by omega. replace (_ + x0 - _) with x0 by omega.
+    pose proof (record_nth_error ?? ?? ?? ?? ?? ** ) as HH.
+    rewrite <- ?map_app.  erewrite map_nth_error with (f := fst); [ | eauto ].
+    reflexivity.
+
+- (* MkClose *) break_bind_state.  econstructor. eapply IHe. eauto.
+
+(* list *)
+- constructor.
+- break_bind_state.
+
+  rename s' into s2, s0 into s1, s into s0.
+  assert (HH : exists s01, s1 = s0 ++ s01) by (eapply compile_state_monotonic; eauto).
+    destruct HH as [s01 Hs01].
+  assert (HH : exists s12, s2 = s1 ++ s12) by (eapply compile_state_monotonic_list; eauto).
+    destruct HH as [s12 Hs12].
+  subst.
+
+  econstructor; eauto.
+  rewrite map_app, app_assoc. eapply I_expr_weaken. eauto.
+
+(* pair *)
+- break_bind_state.  split; eauto.
+
+(* list_pair *)
+- constructor.
+- break_bind_state.
+
+  rename s' into s2, s0 into s1, s into s0.
+  assert (HH : exists s01, s1 = s0 ++ s01) by (eapply compile_state_monotonic_pair; eauto).
+    destruct HH as [s01 Hs01].
+  assert (HH : exists s12, s2 = s1 ++ s12) by (eapply compile_state_monotonic_list_pair; eauto).
+    destruct HH as [s12 Hs12].
+  subst.
+
+  econstructor; eauto.
+  specialize (IHe ?? ?? ?? ?? **). destruct IHe.
+  split; eauto.
+  rewrite map_app, app_assoc. eapply I_expr_weaken_pair. eauto.
+
+Qed.
+
+
+
+
+Ltac B_start HS :=
+    match goal with
+    | [ |- context [ ?pred ?E ?s _ ] ] =>
+            lazymatch pred with
+            | B.sstep => idtac
+            | B.sstar => idtac
+            | B.splus => idtac
+            | _ => fail "unrecognized predicate:" pred
+            end;
+            let S_ := fresh "S" in
+            let S0 := fresh "S" in
+            set (S0 := s);
+            change s with S0;
+            assert (HS : B.sstar E S0 S0) by (eapply B.SStarNil)
+    end.
+
+Ltac B_step HS :=
+    let S_ := fresh "S" in
+    let S2 := fresh "S" in
+    let HS' := fresh HS "'" in
+    let go E s0 s1 Brel solver :=
+        rename HS into HS';
+        evar (S2 : B.state);
+        assert (HS : Brel E s0 S2);
+        [ solver; unfold S2
+        | clear HS' ] in
+    match type of HS with
+    | B.sstar ?E ?s0 ?s1 => go E s0 s1 B.splus
+            ltac:(eapply sstar_then_splus with (1 := HS');
+                  eapply B.SPlusOne)
+    | B.splus ?E ?s0 ?s1 => go E s0 s1 B.splus
+            ltac:(eapply splus_snoc with (1 := HS'))
+    end.
+
+Ltac B_star HS :=
+    let S_ := fresh "S" in
+    let S2 := fresh "S" in
+    let HS' := fresh HS "'" in
+    let go E s0 s1 Brel solver :=
+        rename HS into HS';
+        evar (S2 : B.state);
+        assert (HS : Brel E s0 S2);
+        [ solver; unfold S2
+        | clear HS' ] in
+    match type of HS with
+    | B.sstar ?E ?s0 ?s1 => go E s0 s1 B.sstar
+            ltac:(eapply sstar_then_sstar with (1 := HS'))
+    | B.splus ?E ?s0 ?s1 => go E s0 s1 B.splus
+            ltac:(eapply splus_then_sstar with (1 := HS'))
+    end.
+
+
+
+
+Require Import Forall3.
+
+Lemma I_expr_map_value : forall BE nfree depth vs bes,
+    Forall2 (I_expr BE nfree depth) (map A.Value vs) bes ->
+    bes = map B.Value vs.
+induction vs; intros0 II; invc II.
+- reflexivity.
+- simpl. f_equal.
+  + on >I_expr, invc. reflexivity.
+  + apply IHvs. eauto.
+Qed.
+
+Lemma locals_list'_length : forall n acc,
+    length (locals_list' n acc) = n + length acc.
+induction n; intros; simpl.
+- reflexivity.
+- rewrite IHn. simpl. omega.
+Qed.
+
+Lemma locals_list_length : forall n,
+    length (locals_list n) = n.
+intros. unfold locals_list. rewrite locals_list'_length. simpl. omega.
+Qed.
+
+Lemma locals_list'_prefix : forall n acc,
+    exists prefix,
+        length prefix = n /\
+        locals_list' n acc = prefix ++ acc.
+induction n; intros; simpl.
+- exists []. split; eauto.
+- specialize (IHn (nth_local n :: acc)). break_exists. break_and.
+  exists (x ++ [nth_local n]). split.
+  + rewrite app_length. simpl. omega.
+  + rewrite <- app_assoc. simpl. auto.
+Qed.
+
+Lemma locals_list'_nth_error : forall n acc i,
+    i < n ->
+    nth_error (locals_list' n acc) i = Some (nth_local i).
+induction n; intros0 Hlt; simpl in *.
+- omega.
+- destruct (eq_nat_dec i n).
+  + subst.
+    fwd eapply locals_list'_prefix with (n := n) (acc := nth_local n :: acc).
+      break_exists. break_and.  on _, fun H => rewrite H.
+    change (?a ++ ?b :: ?c) with (a ++ [b] ++ c).
+    rewrite app_assoc. 
+    rewrite nth_error_app1 by (rewrite app_length; simpl; omega).
+    rewrite nth_error_app2 by omega.
+    replace (n - length x) with 0 by omega.
+    reflexivity.
+  + rewrite IHn; eauto. omega.
+Qed.
+
+Lemma locals_list_nth_error : forall n i,
+    i < n ->
+    nth_error (locals_list n) i = Some (nth_local i).
+intros. unfold locals_list. rewrite locals_list'_nth_error; eauto.
+Qed.
+
+Lemma nth_local_not_value : forall i, ~ B.is_value (nth_local i).
+destruct i; inversion 1.
+Qed.
+
+Lemma crunch_nth_local : forall BE i l k v,
+    nth_error l i = Some v ->
+    B.sstep BE (B.Run (nth_local i) l k) (k v).
+destruct i; intros0 Hnth; simpl.
+- eapply B.SArg. auto.
+- eapply B.SUpVar. auto.
+Qed.
+
+Lemma nth_error_split : forall A i (xs : list A) x,
+    nth_error xs i = Some x ->
+    xs = firstn i xs ++ [x] ++ skipn (S i) xs.
+induction i; intros0 Hnth; simpl in *.
+- break_match; try discriminate. congruence.
+- break_match; try discriminate. simpl.
+  erewrite <- IHi; eauto.
+Qed.
+
+Lemma crunch_MkClose_locals_list' : forall BE fname l k j i es,
+    j <= length l ->
+    i = length l - j ->
+    sliding i (map B.Value l) (locals_list (length l)) es ->
+    B.sstar BE
+        (B.Run (B.MkClose fname es) l k)
+        (B.Run (B.MkClose fname (map B.Value l)) l k).
+induction j; intros0 Hj Hi Hsl.
+
+  { replace i with (length l) in Hsl by omega.
+    erewrite <- map_length in Hsl at 1.
+    fwd eapply sliding_all_eq; eauto.
+      { rewrite map_length, locals_list_length. omega. }
+    subst. eapply B.SStarNil. }
+
+assert (length es = length l).
+  { erewrite <- map_length with (l := l).  eapply sliding_length; [ | eauto].
+    rewrite map_length, locals_list_length. reflexivity. }
+assert (i < length l) by omega.
+assert (i < length es) by omega.
+
+destruct (nth_error es i) eqn:Hnth; cycle 1.
+  { contradict Hnth. rewrite nth_error_Some. auto. }
+destruct (nth_error l i) eqn:Hnth'; cycle 1.
+  { contradict Hnth'. rewrite nth_error_Some. auto. }
+
+fwd eapply nth_error_split with (xs := es) as Hes; eauto.
+  rewrite Hes.
+(*
+fwd eapply sliding_next; [ | eassumption | | ]; try eassumption.
+  { eapply map_nth_error. eassumption. }
+  *)
+
+assert (e = nth_local i).
+  { unfold sliding in Hsl. destruct Hsl.
+    replace i with (i + 0) in Hnth by omega. rewrite <- skipn_nth_error in Hnth.
+    on (skipn _ _ = _), fun H => rewrite H in Hnth. rewrite skipn_nth_error in Hnth.
+    replace (i + 0) with i in Hnth by omega. rewrite locals_list_nth_error in Hnth by auto.
+    inject_some. congruence. }
+  subst e.
+
+B_start HS.
+
+B_step HS.
+  { eapply B.SCloseStep.
+    + unfold sliding in Hsl. break_and.
+      on (firstn _ _ = _), fun H => rewrite H.
+      eapply Forall_firstn. eapply Forall_map_intro.
+      eapply Forall_forall. intros. constructor.
+    + eapply nth_local_not_value.
+  }
+
+B_step HS.
+  { eapply crunch_nth_local. eauto. }
+
+B_star HS.
+  { eapply IHj.
+    - omega.
+    - reflexivity.
+    - replace (length l - j) with (S i) by omega.  eapply sliding_next; eauto.
+      eapply map_nth_error. auto.
+  }
+
+eapply splus_sstar.  exact HS.
+Qed.
+
+Lemma crunch_MkClose_locals_list : forall BE fname l k,
+    B.sstar BE
+        (B.Run (B.MkClose fname (locals_list (length l))) l k)
+        (B.Run (B.MkClose fname (map B.Value l)) l k).
+intros. eapply crunch_MkClose_locals_list' with (i := 0) (j := length l).
+- eauto.
+- omega.
+- eapply sliding_zero.
+Qed.
+
+Lemma unroll_elim_length : forall case args rec mk_rec e',
+    A.unroll_elim case args rec mk_rec = Some e' ->
+    length args = length rec.
+first_induction args; destruct rec; intros0 Hunroll; try discriminate; simpl in *.
+- reflexivity.
+- f_equal. eauto.
+Qed.
+
+Lemma unroll_elim_ok : forall case args rec mk_rec,
+    length args = length rec ->
+    exists e', B.unroll_elim case args rec mk_rec = Some e'.
+first_induction args; destruct rec; intros0 Hlen; try discriminate; simpl in *.
+- eauto.
+- remember (if b then _ else _) as case'.
+  specialize (IHargs case' rec mk_rec ltac:(lia)). eauto.
+Qed.
+Lemma unroll_elim_sim : forall BE nfree depth,
+    forall acase bcase args rec amk_rec bmk_rec ae' be',
+    I_expr BE nfree depth acase bcase ->
+    (forall ae be,
+        I_expr BE nfree depth ae be ->
+        I_expr BE nfree depth (amk_rec ae) (bmk_rec be)) ->
+    A.unroll_elim acase args rec amk_rec = Some ae' ->
+    B.unroll_elim bcase args rec bmk_rec = Some be' ->
+    I_expr BE nfree depth ae' be'.
+first_induction args; intros0 Hcase Hmk_rec Aunroll Bunroll;
+destruct rec; try discriminate; simpl in *.
+  { inject_some. assumption. }
+
+rename a into arg.
+eapply IHargs with (3 := Aunroll) (4 := Bunroll); try eassumption.
+destruct b; eauto using ICall, IValue.
+Qed.
+
+
+Lemma I_expr_value : forall BE nfree depth a b,
+    I_expr BE nfree depth a b ->
+    A.is_value a ->
+    B.is_value b.
+intros0 II Aval. invc Aval. invc II. constructor.
+Qed.
+Hint Resolve I_expr_value.
+
+Lemma I_expr_value' : forall BE nfree depth a b,
+    I_expr BE nfree depth a b ->
+    B.is_value b ->
+    A.is_value a.
+intros0 II Bval. invc Bval. invc II. constructor.
+Qed.
+Hint Resolve I_expr_value'.
+
+Lemma I_expr_not_value : forall BE nfree depth a b,
+    I_expr BE nfree depth a b ->
+    ~ A.is_value a ->
+    ~ B.is_value b.
+intros0 II Aval. contradict Aval. eauto using I_expr_value'.
+Qed.
+Hint Resolve I_expr_not_value.
+
+Lemma I_expr_not_value' : forall BE nfree depth a b,
+    I_expr BE nfree depth a b ->
+    ~ B.is_value b ->
+    ~ A.is_value a.
+intros0 II Bval. contradict Bval. eauto using I_expr_value.
+Qed.
+Hint Resolve I_expr_not_value'.
+
+
+Ltac i_ctor := intros; econstructor; simpl; eauto.
+Ltac i_lem H := intros; eapply H; simpl; eauto.
+
+Theorem I_sim : forall AE BE0 BE1 NFREES a a' b,
+    Forall3 (fun a b nfree => I_expr (BE0 ++ BE1) nfree 0 a b) AE BE0 NFREES ->
+    I AE (BE0 ++ BE1) a b ->
+    A.sstep AE a a' ->
+    exists b',
+        B.splus (BE0 ++ BE1) b b' /\
+        I AE (BE0 ++ BE1) a' b'.
+destruct a as [ae al ak | av]; cycle 1.
+  { intros0 Henv II Astep. invc Astep. }
+generalize dependent ak. generalize dependent al.
+induction ae using A.expr_ind''; intros0 Henv II Astep;
+invc Astep; invc II; try on (I_expr _ _ _ _ _), invc;
+simpl in *.
+
+- (* SArg *)
+  break_match; try discriminate. inject_some.
+  destruct bextra; try discriminate.
+
+  eexists. split. eapply B.SPlusOne; i_lem B.SArg.
+  auto.
+
+- (* SArg -> SUpVar *)
+  break_match; try discriminate. inject_some.
+
+  eexists. split. eapply B.SPlusOne; eapply B.SUpVar.
+  + replace (S depth) with (length bextra + 0) by lia.
+    rewrite nth_error_app2 by lia. replace (_ + 0 - _) with 0 by lia.
+    reflexivity.
+  + auto.
+
+- (* SUpVar *)
+  break_match; try discriminate. inject_some.
+
+  eexists. split. eapply B.SPlusOne; eapply B.SUpVar.
+  + replace (S _) with (length bextra + S n) by lia.
+    rewrite nth_error_app2 by lia. replace (_ + _ - _) with (S n) by lia.
+    simpl. eauto.
+  + auto.
+
+- (* SCallL *)
+  eexists. split. eapply B.SPlusOne; i_lem B.SCallL.
+  i_ctor. i_ctor. i_ctor; [i_ctor|].
+  rewrite Nat.add_0_r. auto.
+
+- (* SCallR *)
+  eexists. split. eapply B.SPlusOne; i_lem B.SCallR.
+  i_ctor. i_ctor. i_ctor; [|i_ctor].
+  rewrite Nat.add_0_r. auto.
+
+- (* SMakeCall *)
+  on (I_expr _ _ _ (A.Value (Close _ _)) _), invc.
+  on (I_expr _ _ _ (A.Value _) _), invc.
+
+  fwd eapply Forall3_length; eauto. break_and.
+  fwd eapply length_nth_error_Some with (ys := BE0); eauto. break_exists.
+  fwd eapply length_nth_error_Some with (ys := NFREES); eauto. break_exists.
+  fwd eapply Forall3_nth_error; eauto. cbv beta in *.
+
+  eexists. split. eapply B.SPlusOne; i_lem B.SMakeCall.
+  + i_lem nth_error_app_Some.
+  + (* on entry to a new function body, we are no longer under any Elims *)
+    eapply IRun with (bextra := []); eauto.
+    admit. (* nfree correctness *)
+
+- (* SConstrStep *)
+  destruct (Forall2_app_inv_l _ _ **) as (? & ? & ? & ? & ?).
+  on (Forall2 _ (_ :: _) _), invc.
+  rename x into b_vs. rename y into b_e. rename l' into b_es.
+
+  eexists. split. eapply B.SPlusOne; i_lem B.SConstrStep.
+  + list_magic_on (vs, (b_vs, tt)).
+  + i_ctor. i_ctor. i_ctor.
+    rewrite Nat.add_0_r. i_lem Forall2_app. i_ctor. i_ctor.
+
+- (* SConstrDone *)
+  fwd eapply I_expr_map_value; eauto. subst.
+  eexists. split. eapply B.SPlusOne; i_lem B.SConstrDone.
+  eauto.
+
+- (* SElimStep *)
+  eexists. split. eapply B.SPlusOne; i_lem B.SElimStep.
+  + i_ctor. i_ctor.
+    rewrite Nat.add_0_r. i_ctor. i_ctor.
+
+- (* SElimStep / SCallL + SMkClose *)
+  B_start HS.
+  B_step HS.  { eapply B.SCallL. inversion 1. }
+  B_star HS.
+    { unfold S1. rewrite <- app_length.
+      eapply crunch_MkClose_locals_list. }
+  B_step HS.  { eapply B.SCloseDone. }
+  B_step HS.  { i_lem B.SCallR. i_ctor. }
+
+  eexists. split. exact HS.
+  + i_ctor. i_lem IMidElim.
+
+- on (~ A.is_value (A.Value _)), contradict. constructor.
+
+- (* SEliminate *)
+  on (I_expr _ _ _ _ btarget), invc.
+  fwd eapply length_nth_error_Some with (ys := bcases) as HH.
+    { eapply Forall2_length. eauto. }
+    { eassumption. }
+    destruct HH as [[bcase brec] Hbcase].
+  fwd eapply Forall2_nth_error with (xs := cases); [eassumption.. |].
+    cbv beta in *. break_and. simpl in *. subst brec.
+  fwd eapply unroll_elim_length; eauto.
+  fwd eapply unroll_elim_ok as HH; eauto.  destruct HH as [be' Hbe'].
+
+  eexists. split. eapply B.SPlusOne; i_lem B.SEliminate.
+  i_ctor.  rewrite Nat.add_0_r.
+  i_lem unroll_elim_sim.  i_ctor.
+
+- (* SEliminate / SMakeCall *)
+  on (I_expr _ _ _ _ btarget), invc.
+  fwd eapply length_nth_error_Some with (ys := bcases) as HH.
+    { eapply Forall2_length. eauto. }
+    { eassumption. }
+    destruct HH as [[bcase brec] Hbcase].
+  fwd eapply Forall2_nth_error with (xs := cases); [eassumption.. |].
+    cbv beta in *. break_and. simpl in *. subst brec.
+  fwd eapply unroll_elim_length; eauto.
+  fwd eapply unroll_elim_ok as HH; eauto.  destruct HH as [be' Hbe'].
+
+  B_start HS.
+  B_step HS.  { eapply B.SCallL. inversion 1. }
+  B_star HS.
+    { unfold S1. rewrite <- app_length.
+      eapply crunch_MkClose_locals_list. }
+  B_step HS.  { eapply B.SCloseDone. }
+  B_step HS.  { eapply B.SMakeCall. eauto. }
+  B_step HS.  { eapply B.SElimStep. inversion 1. }
+  B_step HS.  { eapply B.SArg. reflexivity. }
+  B_step HS.  { i_lem B.SEliminate. }
+
+  eexists. split. exact HS.
+  eapply IRun with (bextra := Constr tag args :: bextra); eauto.
+  rewrite Nat.add_0_r. i_lem unroll_elim_sim. i_ctor.
+
+- (* IMidElim - SEliminate / SMakeCall *)
+  fwd eapply length_nth_error_Some with (ys := bcases) as HH.
+    { eapply Forall2_length. eauto. }
+    { eassumption. }
+    destruct HH as [[bcase brec] Hbcase].
+  fwd eapply Forall2_nth_error with (xs := cases); [eassumption.. |].
+    cbv beta in *. break_and. simpl in *. subst brec.
+  fwd eapply unroll_elim_length; eauto.
+  fwd eapply unroll_elim_ok as HH; eauto.  destruct HH as [be' Hbe'].
+
+  B_start HS.
+  B_step HS.  { eapply B.SMakeCall. eauto. }
+  B_step HS.  { eapply B.SElimStep. inversion 1. }
+  B_step HS.  { eapply B.SArg. reflexivity. }
+  B_step HS.  { i_lem B.SEliminate. }
+
+  eexists. split. exact HS.
+  eapply IRun with (bextra := Constr tag args :: bextra); eauto.
+  rewrite Nat.add_0_r. i_lem unroll_elim_sim. i_ctor.
+
+- (* SCloseStep *)
+  destruct (Forall2_app_inv_l _ _ **) as (? & ? & ? & ? & ?).
+  on (Forall2 _ (_ :: _) _), invc.
+  rename x into b_vs. rename y into b_e. rename l' into b_es.
+
+  eexists. split. eapply B.SPlusOne; i_lem B.SCloseStep.
+  + list_magic_on (vs, (b_vs, tt)).
+  + i_ctor. i_ctor. i_ctor.
+    rewrite Nat.add_0_r. i_lem Forall2_app. i_ctor. i_ctor.
+
+- (* SCloseDone *)
+  fwd eapply I_expr_map_value; eauto. subst.
+  eexists. split. eapply B.SPlusOne; i_lem B.SCloseDone.
+  eauto.
+
+- 
+
+Qed.
+
+
+
+
+
+
+
+  (* TODO *)
+
+
+      - 
+
+  E_star HS.
+    { eapply E_call_close_dyn_either; eauto. }
+
+  E_step HS.
+    { eapply B.SCallR.
+      - constructor.
+      - eapply I_expr_not_value; eauto. }
+
+  eexists. split. eassumption.
+  constructor; eauto.
+  intros. constructor; eauto.
+  econstructor; eauto using T_value_I_expr_locals.
+
+- (* SEliminate *)
+  B_start HS.
+
+  (* we start at the B.Call *)
+
+  (* eval closure *)
+  E_star HS.
+    { eapply E_call_close_dyn_either; eauto. }
+
+  (* make the call *)
+  on (I_expr _ _ _ _ etarget), invc.
+  E_step HS.
+    { eapply B.SMakeCall; eauto. }
+
+  (* now we are at the B.ElimBody *)
+
+  (* eval rec *)
+  E_step HS. { eapply B.SElimStepRec. inversion 1. }
+  E_step HS. { eapply B.SCloseDyn. } simpl in S4.
+
+  (* enter the case *)
+  remember (compile_list_pair _ _) as ecases.
+  assert (length ecases = length cases). {
+    subst ecases. rewrite compile_list_pair_length. reflexivity.
+  }
+  fwd eapply length_nth_error_Some with (xs := cases) (ys := ecases); eauto.
+    destruct ** as [[ecase erec] ?].
+  assert ((ecase, erec) = compile_pair (length TE) (case, rec)). {
+    on (_ = compile_list_pair _ _), fun H => (symmetry in H;
+        eapply compile_list_pair_Forall_fwd in H).
+    remember (case, rec) as tp. remember (ecase, erec) as ep.
+    symmetry.
+    eapply Forall2_nth_error with (P := fun tp ep => compile_pair _ tp = ep); eauto.
+  }
+  assert (length args = length rec) by (eauto using T_unroll_elim_length).
+  assert (erec = rec) by (simpl in *; congruence).
+  (*assert (length eargs = length args) by (symmetry; eauto using Forall2_length).*)
+  (*assert (length eargs = length erec) by congruencB.*)
+  fwd eapply E_unroll_elim_ok; eauto. destruct ** as (ee' & ?).
+  E_step HS.
+    { eapply B.SEliminatB.
+      - constructor.
+      - eassumption.
+      - subst rec. eassumption.
+    }
+
+  eexists. split. eapply HS. unfold S5.
+  constructor; eauto.
+  eapply unroll_elim_sim.
+  3: reflexivity.
+  4: eassumption.
+  4: eassumption.
+  1: eauto.
+  + cbn [compile_pair] in *. inject_pair.
+    eapply compile_I_expr; eauto.
+    invc Helims'.  on (A.elims_match _ _), fun H => simpl in H.
+      A.refold_elims_match ELIMS.  break_and.
+    rewrite A.elims_match_list_pair_Forall in *.
+    assert (A.elims_match_pair ELIMS (case, rec)).  { eapply Forall_nth_error; eauto. }
+    on >A.elims_match_pair, fun H => simpl in H. auto.
+  + simpl. intros0 IE'. econstructor.
+    * reflexivity.
+    * eassumption.
+    * reflexivity.
+    * assumption.
+    * right. reflexivity.
+    * assumption.
+
+- destruct (Forall2_app_inv_l _ _ **) as (? & ? & ? & ? & ?).
+  on (Forall2 _ (_ :: _) _), invc.
+  rename x into e_vs. rename y into e_B. rename l' into e_es.
+
+  eexists. split. eapply B.SPlusOne, B.SCloseStep.
+  + list_magic_on (vs, (e_vs, tt)). eauto using I_expr_valuB.
+  + eauto using I_expr_value'.
+  + constructor; eauto.
+    intros. constructor; eauto.
+    constructor. eapply Forall2_app; eauto. constructor; eauto using T_value_I_expr_locals.
+
+  - fwd eapply I_expr_map_value; eauto. subst.
+
+  eexists. split. eapply B.SPlusOne, B.SCloseDonB.
+  eauto.
+
+Qed.
+
+
+simpl in *.
+
+
+(* TODO *)
+Inductive I_expr (BE : B.env) nfree : nat -> A.expr -> B.expr -> Prop :=
+
+  
 
 
 
